compiler1/semantics/exhPropsScript.sml
@@ -48,4 +48,62 @@ val build_rec_env_merge = store_thm("build_rec_env_merge",
 
 val Boolv_disjoint = save_thm("Boolv_disjoint",EVAL``exhSem$Boolv T = Boolv F``);
 
+val pmatch_any_match = store_thm("pmatch_any_match",
+  ``(∀s p v env env'. pmatch s p v env = Match env' ⇒
+       ∀env. ∃env'. pmatch s p v env = Match env') ∧
+    (∀s ps vs env env'. pmatch_list s ps vs env = Match env' ⇒
+       ∀env. ∃env'. pmatch_list s ps vs env = Match env')``,
+  ho_match_mp_tac pmatch_ind >>
+  rw[pmatch_def] >>
+  pop_assum mp_tac >>
+  BasicProvers.CASE_TAC >>
+  fs[] >> strip_tac >> fs[] >>
+  BasicProvers.CASE_TAC >> fs[] >>
+  metis_tac[semanticPrimitivesTheory.match_result_distinct])
+
+val pmatch_any_no_match = store_thm("pmatch_any_no_match",
+  ``(∀s p v env. pmatch s p v env = No_match ⇒
+       ∀env. pmatch s p v env = No_match) ∧
+    (∀s ps vs env. pmatch_list s ps vs env = No_match ⇒
+       ∀env. pmatch_list s ps vs env = No_match)``,
+  ho_match_mp_tac pmatch_ind >>
+  rw[pmatch_def] >>
+  pop_assum mp_tac >>
+  BasicProvers.CASE_TAC >>
+  fs[] >> strip_tac >> fs[] >>
+  BasicProvers.CASE_TAC >> fs[] >>
+  imp_res_tac pmatch_any_match >>
+  metis_tac[semanticPrimitivesTheory.match_result_distinct])
+
+val pmatch_any_match_error = store_thm("pmatch_any_match_error",
+  ``(∀s p v env. pmatch s p v env = Match_type_error ⇒
+       ∀env. pmatch s p v env = Match_type_error) ∧
+    (∀s ps vs env. pmatch_list s ps vs env = Match_type_error ⇒
+       ∀env. pmatch_list s ps vs env = Match_type_error)``,
+  rw[] >> qmatch_abbrev_tac`X = Y` >> Cases_on`X` >> fs[markerTheory.Abbrev_def] >>
+  metis_tac[semanticPrimitivesTheory.match_result_distinct
+           ,pmatch_any_no_match,pmatch_any_match]);
+
+val pmatch_list_pairwise = store_thm("pmatch_list_pairwise",
+  ``∀ps vs s env env'. pmatch_list s ps vs env = Match env' ⇒
+      EVERY2 (λp v. ∀env. ∃env'. pmatch s p v env = Match env') ps vs``,
+  Induct >> Cases_on`vs` >> simp[pmatch_def] >>
+  rpt gen_tac >> BasicProvers.CASE_TAC >> strip_tac >>
+  res_tac >> simp[] >> metis_tac[pmatch_any_match])
+
+val _ = store_thm("pmatch_list_snoc_nil[simp]",
+  ``∀p ps v vs s env.
+      (pmatch_list s [] (SNOC v vs) env = Match_type_error) ∧
+      (pmatch_list s (SNOC p ps) [] env = Match_type_error)``,
+  Cases_on`ps`>>Cases_on`vs`>>simp[pmatch_def]);
+
+val pmatch_list_snoc = store_thm("pmatch_list_snoc",
+  ``∀ps vs p v s env. LENGTH ps = LENGTH vs ⇒
+      pmatch_list s (SNOC p ps) (SNOC v vs) env =
+      case pmatch_list s ps vs env of
+      | Match env' => pmatch s p v env'
+      | res => res``,
+  Induct >> Cases_on`vs` >> simp[pmatch_def] >> rw[] >>
+  BasicProvers.CASE_TAC)
+
 val _ = export_theory()
